MPL/ProofMode/Tactics/Exact.lean
@@ -12,8 +12,8 @@ open Lean Elab Tactic Meta
 theorem Exact.assumption {σs : List Type} {P P' A : SPred σs}
   (h : P ⊣⊢ₛ P' ∧ A) : P ⊢ₛ A := h.mp.trans SPred.and_elim_r
 
-theorem Exact.from_tautology {σs : List Type} {P T : SPred σs} (htaut : ⊢ₛ T) : P ⊢ₛ T :=
-  SPred.true_intro.trans htaut
+theorem Exact.from_tautology {σs : List Type} {P T : SPred σs} [PropAsSPredTautology φ T] (h : φ) : P ⊢ₛ T :=
+  SPred.true_intro.trans (PropAsSPredTautology.iff.mp h)
 
 def _root_.MPL.ProofMode.MGoal.exact (goal : MGoal) (hyp : TSyntax `term) : OptionT MetaM Expr := do
   let some focusRes := goal.focusHyp hyp.raw.getId | failure
@@ -24,12 +24,12 @@ def _root_.MPL.ProofMode.MGoal.exact (goal : MGoal) (hyp : TSyntax `term) : Opti
   return proof
 
 def _root_.MPL.ProofMode.MGoal.exactPure (goal : MGoal) (hyp : TSyntax `term) : TacticM Expr := do
-  let T := goal.target
-  let expected := mkApp2 (mkConst ``SPred.tautological) goal.σs T
-  let prf ← try
-    elabTerm hyp expected
-  catch _ => throwError "mexact tactic failed, {hyp} does not have type {expected}"
-  return mkApp4 (mkConst ``Exact.from_tautology) goal.σs goal.hyps goal.target prf
+  let φ ← mkFreshExprMVar (mkSort .zero)
+  let h ← elabTermEnsuringType hyp φ
+  let P ← mkFreshExprMVar (mkApp (mkConst ``SPred) goal.σs)
+  let some inst ← synthInstance? (mkApp3 (mkConst ``PropAsSPredTautology) φ goal.σs P)
+    | throwError "mexact tactic failed, {hyp} is not an SPred tautology"
+  return mkApp6 (mkConst ``Exact.from_tautology) φ goal.σs goal.hyps goal.target inst h
 
 elab "mexact" colGt hyp:term : tactic => do
   let mvar ← getMainGoal
